some helper lemmas about slice

theories/logrel/logrel_prim.v
@@ -2,7 +2,7 @@ From iris.proofmode Require Import tactics.
 From machine_program_logic.program_logic Require Import weakestpre.
 From HypVeri.lang Require Import lang.
 From HypVeri.algebra Require Import base base_extra mem mailbox trans.
-From HypVeri.logrel Require Export logrel logrel_extra.
+From HypVeri.logrel Require Export logrel logrel_extra big_sepSS.
 
 Section logrel_prim.
 
@@ -17,22 +17,22 @@ Section logrel_prim.
           ((tran.1.1.1.1 = V0 ∧ tran.1.2 ≠ Donation) -> ∃ tran', trans' !! h = Some tran' ∧ tran.1 = tran'.1)
      ) trans.
 
-  Definition transaction_pagetable_entries_transferred_all (trans: gmap Addr transaction) : iProp Σ:=
-    big_sepFM trans (λ kv, kv.2.1.2 = Donation) (λ k v, k -{1/4}>t v.1 ∗ pgt_1_4 v.1.1.2 v.1.1.1.1 true)%I.
+  (* Definition transaction_pagetable_entries_transferred_all (trans: gmap Addr transaction) : iProp Σ:= *)
+  (*   big_sepFM trans (λ kv, kv.2.1.2 = Donation) (λ k v, k -{1/4}>t v.1 ∗ pgt_1_4 v.1.1.2 v.1.1.1.1 true)%I. *)
 
-  Definition retrievable_transaction_transferred_all(trans: gmap Addr transaction) : iProp Σ:=
-    (big_sepFM trans (λ kv, True) (λ k v, k -{1/2}>re v.2 )%I) ∗
-    (big_sepFM trans (λ kv, kv.2.2 = false) (λ k v, k -{1/4}>t v.1 ∗ k -{1/2}>re v.2)%I).
+  (* Definition retrievable_transaction_transferred_all(trans: gmap Addr transaction) : iProp Σ:= *)
+  (*   (big_sepFM trans (λ kv, True) (λ k v, k -{1/2}>re v.2 )%I) ∗ *)
+  (*   (big_sepFM trans (λ kv, kv.2.2 = false) (λ k v, k -{1/4}>t v.1 ∗ k -{1/2}>re v.2)%I). *)
 
-  Definition transaction_pagetable_entries_transferred_except (i: VMID) (trans: gmap Addr transaction) : iProp Σ:=
-    big_sepFM trans (λ kv, kv.2.1.2 = Donation ∧ ¬(kv.2.1.1.1.1 = i ∨ kv.2.1.1.1.2 = i)) (λ k v, k -{1/4}>t v.1 ∗ pgt_1_4 v.1.1.2 v.1.1.1.1 true)%I.
+  (* Definition transaction_pagetable_entries_transferred_except (i: VMID) (trans: gmap Addr transaction) : iProp Σ:= *)
+  (*   big_sepFM trans (λ kv, kv.2.1.2 = Donation ∧ ¬(kv.2.1.1.1.1 = i ∨ kv.2.1.1.1.2 = i)) (λ k v, k -{1/4}>t v.1 ∗ pgt_1_4 v.1.1.2 v.1.1.1.1 true)%I. *)
 
-  Definition retrievable_transaction_transferred_except (i: VMID) (trans: gmap Addr transaction) : iProp Σ:=
-    (big_sepFM trans (λ kv, ¬(kv.2.1.1.1.1 = i ∨ kv.2.1.1.1.2 = i)) (λ k v, k -{1/2}>re v.2 )%I) ∗
-    (big_sepFM trans (λ kv, ¬(kv.2.1.1.1.1 = i ∨ kv.2.1.1.1.2 = i) ∧ kv.2.2 = false) (λ k v, k -{1/4}>t v.1 ∗ k -{1/2}>re v.2)%I).
+  (* Definition retrievable_transaction_transferred_except (i: VMID) (trans: gmap Addr transaction) : iProp Σ:= *)
+  (*   (big_sepFM trans (λ kv, ¬(kv.2.1.1.1.1 = i ∨ kv.2.1.1.1.2 = i)) (λ k v, k -{1/2}>re v.2 )%I) ∗ *)
+  (*   (big_sepFM trans (λ kv, ¬(kv.2.1.1.1.1 = i ∨ kv.2.1.1.1.2 = i) ∧ kv.2.2 = false) (λ k v, k -{1/4}>t v.1 ∗ k -{1/2}>re v.2)%I). *)
 
-  Definition transferred_memory_pages_all (trans : gmap Word transaction) :=
-    pages_in_trans (filter (λ kv, ¬(kv.2.2 = true ∧ kv.2.1.2 = Lending)) trans).
+  (* Definition transferred_memory_pages_all (trans : gmap Word transaction) := *)
+  (*   pages_in_trans (filter (λ kv, ¬(kv.2.2 = true ∧ kv.2.1.2 = Lending)) trans). *)
 
   Definition transferred_memory_pages_slice (j: VMID) (i:VMID) (trans : gmap Addr transaction) :=
     pages_in_trans (filter (λ kv, (kv.2.1.1.1.1 = i ∧ kv.2.1.1.1.2 = j) ∧ ¬(kv.2.2 = true ∧ kv.2.1.2 = Lending)) trans).
@@ -46,9 +46,13 @@ Section logrel_prim.
 
   Definition set_of_vmids : gset VMID := (list_to_set list_of_vmids).
 
+  Definition slice_wf (Φ: (gmap Addr transaction) -> (VMID * VMID)-> iProp Σ) :=
+    ∀ i j trans trans', map_Forall (λ h tran, tran.1.1.1.1 = i ∧ tran.1.1.1.2 = j -> ∃ tran', trans' !! h = Some tran' ∧ tran = tran') trans ->
+    (Φ trans (i,j) ⊣⊢ Φ trans' (i,j)).
+
   Program Definition interp_access_prim p_tx p_rx ps_acc trans (Φ: (gmap Addr transaction) -> (VMID * VMID)-> iProp Σ): iPropO Σ:=
     (
-      let ps_macc_trans := (transferred_memory_pages_all trans) in
+      (* let ps_macc_trans := (transferred_memory_pages_all trans) in *)
       let ps_oea := ps_acc ∖ {[p_rx;p_tx]} ∖ (currently_accessible_in_trans_memory_pages V0 trans) in
       (∃ regs, ⌜is_total_gmap regs⌝ ∗ [∗ map] r ↦ w ∈ regs, r @@ V0 ->r w) ∗
       (tx_page V0 p_tx ∗ ∃ mem_tx, memory_page p_tx mem_tx) ∗
@@ -63,10 +67,10 @@ Section logrel_prim.
       (∃ rx_state, RX_state@ V0 := rx_state) ∗ (rx_page V0 p_rx) ∗ (∃ mem_rx, memory_page p_rx mem_rx) ∗
       transaction_hpool_global_transferred trans ∗
       rx_pages (list_to_set (list_of_vmids) ∖ {[V0]}) ∗
-      ([∗ set] i ∈ set_of_vmids, [∗ set] j ∈ set_of_vmids, Φ trans (i,j)) ∗
-      transaction_pagetable_entries_transferred_all trans ∗
-      retrievable_transaction_transferred_all trans ∗
-      (∃ mem_trans, memory_pages ps_macc_trans mem_trans) ∗
+      (big_sepSS set_of_vmids (Φ trans)) ∗
+      (* transaction_pagetable_entries_transferred_all trans ∗ *)
+      (* retrievable_transaction_transferred_all trans ∗ *)
+      (* (∃ mem_trans, memory_pages ps_macc_trans mem_trans) ∗ *)
       [∗ set] i ∈ set_of_vmids ∖ {[V0]}, VMProp (i:VMID) (vmprop_unknown i p_tx p_rx) (1/2)%Qp
     )%I.
 
